fstar/new/MLS.TreeDEM.Message.Framing.fst
@@ -70,19 +70,7 @@ noeq type encrypted_sender_data_content = {
   reuse_guard: lbytes 4;
 }
 
-val message_plaintext_to_message: message_plaintext -> message & message_auth
-let message_plaintext_to_message pt =
-  (({
-    group_id = pt.group_id;
-    epoch = pt.epoch;
-    sender = pt.sender;
-    authenticated_data = pt.authenticated_data;
-    content_type = pt.content_type;
-    message_content = pt.message_content;
-  } <: message), ({
-    signature = pt.signature;
-    confirmation_tag = pt.confirmation_tag;
-  } <: message_auth))
+(*** From/to network ***)
 
 val network_to_sender_type: sender_type_nt -> result sender_type
 let network_to_sender_type s =
@@ -154,6 +142,33 @@ let network_to_message_plaintext pt =
     membership_tag = membership_tag;
   } <: message_plaintext)
 
+val message_plaintext_to_network: ciphersuite -> message_plaintext -> result mls_plaintext_nt
+let message_plaintext_to_network cs pt =
+  if not (Seq.length pt.group_id < 256) then
+    error "message_plaintext_to_network: group_id too long"
+  else if not (pt.epoch < pow2 64) then
+    error "message_plaintext_to_network: epoch too big"
+  else if not (Seq.length pt.authenticated_data < pow2 32) then
+    error "message_plaintext_to_network: authenticated_data too long"
+  else if not (Seq.length pt.signature < pow2 16) then
+    error "message_plaintext_to_network: signature too long"
+  else (
+    sender <-- sender_to_network pt.sender;
+    content <-- message_content_pair_to_network cs pt.message_content;
+    confirmation_tag <-- opt_bytes_to_opt_tag pt.confirmation_tag;
+    membership_tag <-- opt_bytes_to_opt_tag pt.membership_tag;
+    return ({
+      group_id = pt.group_id;
+      epoch = u64 pt.epoch;
+      sender = sender;
+      authenticated_data = pt.authenticated_data;
+      content = content;
+      signature = pt.signature;
+      confirmation_tag = confirmation_tag;
+      membership_tag = membership_tag;
+    } <: mls_plaintext_nt)
+  )
+
 val network_to_ciphertext_content: #content_type: content_type_nt{valid_network_message_content_type content_type} -> mls_ciphertext_content_nt content_type -> result (message_ciphertext_content (network_to_message_content_type_tot content_type))
 let network_to_ciphertext_content #content_type ciphertext_content =
   content <-- network_to_message_content ciphertext_content.content;
@@ -162,8 +177,197 @@ let network_to_ciphertext_content #content_type ciphertext_content =
     message_content = content;
     signature = ciphertext_content.signature;
     confirmation_tag = confirmation_tag;
-    padding = ciphertext_content.signature;
+    padding = ciphertext_content.padding;
   })
+
+val ciphertext_content_to_network: #content_type: message_content_type -> ciphersuite -> message_ciphertext_content content_type -> result (mls_ciphertext_content_nt (message_content_type_to_network content_type))
+let ciphertext_content_to_network #content_type cs content =
+  if not (Seq.length content.signature < pow2 16) then
+    internal_failure "ciphertext_content_to_network: signature too long"
+  else if not (Seq.length content.padding < pow2 16) then
+    internal_failure "ciphertext_content_to_network: padding too long"
+  else (
+    network_content <-- message_content_to_network cs content.message_content;
+    confirmation_tag <-- opt_bytes_to_opt_tag content.confirmation_tag;
+    return ({
+      content = network_content;
+      signature = content.signature;
+      confirmation_tag = confirmation_tag;
+      padding = content.padding;
+    } <: mls_ciphertext_content_nt (message_content_type_to_network content_type))
+  )
+
+val network_to_encrypted_sender_data: mls_sender_data_nt -> encrypted_sender_data_content
+let network_to_encrypted_sender_data sd =
+  ({
+    sender = Lib.IntTypes.v sd.sender;
+    generation = Lib.IntTypes.v sd.generation;
+    reuse_guard = sd.reuse_guard;
+  })
+
+val encrypted_sender_data_to_network: encrypted_sender_data_content -> result mls_sender_data_nt
+let encrypted_sender_data_to_network sd =
+  if not (sd.sender < pow2 32) then
+    internal_failure "encrypted_sender_data_to_network: sender too big"
+  else if not (sd.generation < pow2 32) then
+    internal_failure "encrypted_sender_data_to_network: generation too big"
+  else
+    return ({
+      sender = u32 sd.sender;
+      generation = u32 sd.generation;
+      reuse_guard = sd.reuse_guard;
+    } <: mls_sender_data_nt)
+
+val network_to_message_ciphertext: mls_ciphertext_nt -> result message_ciphertext
+let network_to_message_ciphertext ct =
+  content_type <-- network_to_message_content_type ct.content_type;
+  return ({
+    group_id = ct.group_id;
+    epoch = Lib.IntTypes.v ct.epoch;
+    content_type = content_type;
+    authenticated_data = ct.authenticated_data;
+    encrypted_sender_data = ct.encrypted_sender_data;
+    ciphertext = ct.ciphertext;
+  })
+
+val message_ciphertext_to_network: message_ciphertext -> result mls_ciphertext_nt
+let message_ciphertext_to_network ct =
+  if not (Seq.length ct.group_id < 256) then
+     internal_failure "message_ciphertext_to_network: group_id too long"
+  else if not (ct.epoch < pow2 64) then
+     internal_failure "message_ciphertext_to_network: epoch too big"
+  else if not (Seq.length ct.authenticated_data < pow2 32) then
+     internal_failure "message_ciphertext_to_network: authenticated_data too long"
+  else if not (Seq.length ct.encrypted_sender_data < 256) then
+     internal_failure "message_ciphertext_to_network: encrypted_sender_data too long"
+  else if not (Seq.length ct.ciphertext < pow2 32) then
+     internal_failure "message_ciphertext_to_network: ciphertext too long"
+  else (
+    return ({
+      group_id = ct.group_id;
+      epoch = u64 ct.epoch;
+      content_type = message_content_type_to_network ct.content_type;
+      authenticated_data = ct.authenticated_data;
+      encrypted_sender_data = ct.encrypted_sender_data;
+      ciphertext = ct.ciphertext;
+    } <: mls_ciphertext_nt)
+  )
+
+(*** Authentication ***)
+
+val compute_message_confirmation_tag: cs:ciphersuite -> bytes -> bytes -> result (lbytes (hash_length cs))
+let compute_message_confirmation_tag cs confirmation_key confirmed_transcript_hash =
+  hmac_hmac cs confirmation_key confirmed_transcript_hash
+
+val compute_tbs: ciphersuite -> message -> result (mls_plaintext_tbs_nt)
+let compute_tbs cs msg =
+  if not (Seq.length msg.group_id < 256) then
+    internal_failure "compute_tbs: group_id too long"
+  else if not (msg.epoch < pow2 64) then
+    internal_failure "compute_tbs: epoch too big"
+  else if not (Seq.length msg.authenticated_data < pow2 32) then
+    internal_failure "compute_tbs: authenticated_data too long"
+  else (
+    sender <-- sender_to_network msg.sender;
+    content <-- message_content_pair_to_network cs msg.message_content;
+    return ({
+      group_id = msg.group_id;
+      epoch = u64 msg.epoch;
+      sender = sender;
+      authenticated_data = msg.authenticated_data;
+      content = content;
+    } <: mls_plaintext_tbs_nt)
+  )
+
+val compute_tbm: ciphersuite -> message -> message_auth -> result (mls_plaintext_tbm_nt)
+let compute_tbm cs msg auth =
+  if not (Seq.length auth.signature < pow2 16) then
+    error "compute_tbm: signature too long"
+  else (
+    tbs <-- compute_tbs cs msg;
+    confirmation_tag' <-- opt_bytes_to_opt_tag auth.confirmation_tag;
+    return ({
+      tbs = tbs;
+      signature = auth.signature;
+      confirmation_tag = confirmation_tag';
+    })
+  )
+
+val compute_tbs_bytes: ciphersuite -> message -> bytes -> result bytes
+let compute_tbs_bytes cs msg group_context =
+  tbs <-- compute_tbs cs msg;
+  let partial_serialized_bytes = ps_mls_plaintext_tbs.serialize tbs in
+  return (
+    if msg.sender.sender_type = ST_member then
+      Seq.append group_context partial_serialized_bytes
+    else
+      partial_serialized_bytes
+  )
+
+val compute_message_signature: cs:ciphersuite -> sign_private_key cs -> randomness (sign_nonce_length cs) -> message -> bytes -> result (sign_signature cs)
+let compute_message_signature cs sk rand msg group_context =
+  serialized_tbs <-- compute_tbs_bytes cs msg group_context;
+  sign_sign cs sk serialized_tbs rand
+
+val check_message_signature: cs:ciphersuite -> sign_public_key cs -> sign_signature cs -> message -> bytes -> result bool
+let check_message_signature cs pk signature msg group_context =
+  serialized_tbs <-- compute_tbs_bytes cs msg group_context;
+  return (sign_verify cs pk serialized_tbs signature)
+
+val compute_message_membership_tag: cs:ciphersuite -> bytes -> message -> message_auth -> bytes -> result (lbytes (hash_length cs))
+let compute_message_membership_tag cs membership_key msg auth group_context =
+  tbm <-- compute_tbm cs msg auth;
+  let partial_serialized_bytes = ps_mls_plaintext_tbm.serialize tbm in
+  let serialized_bytes =
+    if msg.sender.sender_type = ST_member then
+      Seq.append group_context partial_serialized_bytes
+    else
+      partial_serialized_bytes
+  in
+  hmac_hmac cs membership_key serialized_bytes
+
+val message_compute_auth: cs:ciphersuite -> message -> sign_private_key cs -> randomness (sign_nonce_length cs) -> group_context:bytes -> bytes -> bytes -> result message_auth
+let message_compute_auth cs msg sk rand group_context confirmation_key confirmed_transcript_hash =
+  signature <-- compute_message_signature cs sk rand msg group_context;
+  confirmation_tag <-- compute_message_confirmation_tag cs confirmation_key confirmed_transcript_hash;
+  return ({
+    signature = signature;
+    confirmation_tag = Some (confirmation_tag);
+  } <: message_auth)
+
+(*** From/to plaintext ***)
+
+//TODO check membership tag?
+val message_plaintext_to_message: message_plaintext -> message & message_auth
+let message_plaintext_to_message pt =
+  (({
+    group_id = pt.group_id;
+    epoch = pt.epoch;
+    sender = pt.sender;
+    authenticated_data = pt.authenticated_data;
+    content_type = pt.content_type;
+    message_content = pt.message_content;
+  } <: message), ({
+    signature = pt.signature;
+    confirmation_tag = pt.confirmation_tag;
+  } <: message_auth))
+
+val message_to_message_plaintext: cs:ciphersuite -> membership_key:bytes -> group_context:bytes -> message & message_auth -> result message_plaintext
+let message_to_message_plaintext cs membership_key group_context (msg, msg_auth) =
+  membership_tag <-- compute_message_membership_tag cs membership_key msg msg_auth group_context;
+  return ({
+    group_id = msg.group_id;
+    epoch = msg.epoch;
+    sender = msg.sender;
+    authenticated_data = msg.authenticated_data;
+    content_type = msg.content_type;
+    message_content = msg.message_content;
+    signature = msg_auth.signature;
+    confirmation_tag = msg_auth.confirmation_tag;
+    membership_tag = Some membership_tag; //TODO when can it be none? (don't have internet atm)
+  } <: message_plaintext)
+
+(*** From/to ciphertext ***)
 
 val get_ciphertext_sample: ciphersuite -> bytes -> bytes
 let get_ciphertext_sample cs ct =
@@ -172,44 +376,92 @@ let get_ciphertext_sample cs ct =
   else
     Seq.slice ct 0 (kdf_length cs)
 
-val decrypt_sender_data: ciphersuite -> message_ciphertext -> bytes -> result mls_sender_data_nt
-let decrypt_sender_data cs ct sender_data_secret =
+
+val message_ciphertext_to_sender_data_aad: message_ciphertext -> result mls_sender_data_aad_nt
+let message_ciphertext_to_sender_data_aad ct =
   if not (Seq.length ct.group_id < 256) then (
-    internal_failure "decrypt_sender_data: group_id too long"
+    internal_failure "message_ciphertext_to_sender_data_aad: group_id too long"
   ) else if not (ct.epoch < pow2 64) then (
-    internal_failure "decrypt_sender_data: epoch too big"
+    internal_failure "message_ciphertext_to_sender_data_aad: epoch too big"
   ) else (
-    let ciphertext_sample = get_ciphertext_sample cs ct.ciphertext in
-    sender_data_key <-- expand_with_label cs sender_data_secret (string_to_bytes "key") ciphertext_sample (aead_key_length cs);
-    sender_data_nonce <-- expand_with_label cs sender_data_secret (string_to_bytes "nonce") ciphertext_sample (aead_nonce_length cs);
-    let ad = ps_mls_sender_data_aad.serialize ({
+    return ({
       group_id = ct.group_id;
       epoch = u64 ct.epoch;
       content_type = message_content_type_to_network ct.content_type;
-    }) in
-    sender_data <-- aead_decrypt cs sender_data_key sender_data_nonce ad ct.encrypted_sender_data;
-    from_option "decrypt_sender_data: malformed sender data" ((ps_to_pse ps_mls_sender_data).parse_exact sender_data)
+    } <: mls_sender_data_aad_nt)
   )
 
-val decrypt_ciphertext_content: cs:ciphersuite -> ct:message_ciphertext -> aead_key cs -> aead_nonce cs -> result (mls_ciphertext_content_nt (message_content_type_to_network ct.content_type))
-let decrypt_ciphertext_content cs ct key nonce =
+//TODO (?): copy-pasted from above
+val message_to_sender_data_aad: message -> result mls_sender_data_aad_nt
+let message_to_sender_data_aad ct =
   if not (Seq.length ct.group_id < 256) then (
-    internal_failure "decrypt_ciphertext_content: group_id too long"
+    internal_failure "message_to_sender_data_aad: group_id too long"
   ) else if not (ct.epoch < pow2 64) then (
-    internal_failure "decrypt_ciphertext_content: epoch too big"
-  ) else if not (Seq.length ct.authenticated_data < pow2 32) then (
-    internal_failure "decrypt_ciphertext_content: authenticated_data too long"
+    internal_failure "message_to_sender_data_aad: epoch too big"
   ) else (
-    let content_type = message_content_type_to_network ct.content_type in
-    let ad = ps_mls_ciphertext_content_aad.serialize ({
+    return ({
       group_id = ct.group_id;
       epoch = u64 ct.epoch;
-      content_type = content_type;
-      authenticated_data = ct.authenticated_data;
-    }) in
-    ciphertext_content <-- aead_decrypt cs key nonce ad ct.ciphertext;
-    from_option "decrypt_ciphertext_content: malformed ciphertext content" ((ps_to_pse (ps_mls_ciphertext_content content_type)).parse_exact ciphertext_content)
+      content_type = message_content_type_to_network ct.content_type;
+    } <: mls_sender_data_aad_nt)
   )
+
+val decrypt_sender_data: cs:ciphersuite -> mls_sender_data_aad_nt -> ciphertext_sample:bytes -> sender_data_secret:bytes -> encrypted_sender_data:bytes -> result mls_sender_data_nt
+let decrypt_sender_data cs ad ciphertext_sample sender_data_secret encrypted_sender_data =
+  sender_data_key <-- expand_with_label cs sender_data_secret (string_to_bytes "key") ciphertext_sample (aead_key_length cs);
+  sender_data_nonce <-- expand_with_label cs sender_data_secret (string_to_bytes "nonce") ciphertext_sample (aead_nonce_length cs);
+  sender_data <-- aead_decrypt cs sender_data_key sender_data_nonce (ps_mls_sender_data_aad.serialize ad) encrypted_sender_data;
+  from_option "decrypt_sender_data: malformed sender data" ((ps_to_pse ps_mls_sender_data).parse_exact sender_data)
+
+val encrypt_sender_data: cs:ciphersuite -> mls_sender_data_aad_nt -> ciphertext_sample:bytes -> sender_data_secret:bytes -> mls_sender_data_nt -> result bytes
+let encrypt_sender_data cs ad ciphertext_sample sender_data_secret sender_data =
+  sender_data_key <-- expand_with_label cs sender_data_secret (string_to_bytes "key") ciphertext_sample (aead_key_length cs);
+  sender_data_nonce <-- expand_with_label cs sender_data_secret (string_to_bytes "nonce") ciphertext_sample (aead_nonce_length cs);
+  aead_encrypt cs sender_data_key sender_data_nonce (ps_mls_sender_data_aad.serialize ad) (ps_mls_sender_data.serialize sender_data)
+
+val message_ciphertext_to_ciphertext_content_aad: ct:message_ciphertext -> result (res:mls_ciphertext_content_aad_nt{res.content_type = message_content_type_to_network ct.content_type})
+let message_ciphertext_to_ciphertext_content_aad ct =
+  if not (Seq.length ct.group_id < 256) then (
+    internal_failure "message_ciphertext_to_ciphertext_content_aad: group_id too long"
+  ) else if not (ct.epoch < pow2 64) then (
+    internal_failure "message_ciphertext_to_ciphertext_content_aad: epoch too big"
+  ) else if not (Seq.length ct.authenticated_data < pow2 32) then (
+    internal_failure "message_ciphertext_to_ciphertext_content_aad: authenticated_data too long"
+  ) else (
+    return ({
+      group_id = ct.group_id;
+      epoch = u64 ct.epoch;
+      content_type = message_content_type_to_network ct.content_type;
+      authenticated_data = ct.authenticated_data;
+    } <: mls_ciphertext_content_aad_nt)
+  )
+
+val decrypt_ciphertext_content: cs:ciphersuite -> ad:mls_ciphertext_content_aad_nt -> aead_key cs -> aead_nonce cs -> ct:bytes -> result (mls_ciphertext_content_nt ad.content_type)
+let decrypt_ciphertext_content cs ad key nonce ct =
+    ciphertext_content <-- aead_decrypt cs key nonce (ps_mls_ciphertext_content_aad.serialize ad) ct;
+    from_option "decrypt_ciphertext_content: malformed ciphertext content" ((ps_to_pse (ps_mls_ciphertext_content ad.content_type)).parse_exact ciphertext_content)
+
+//TODO (?): copy-pasted from message_ciphertext_to_ciphertext_content_aad, can we simplify?
+val message_to_ciphertext_content_aad: msg:message -> result (res:mls_ciphertext_content_aad_nt{res.content_type = message_content_type_to_network msg.content_type})
+let message_to_ciphertext_content_aad msg =
+  if not (Seq.length msg.group_id < 256) then (
+    internal_failure "message_to_ciphertext_content_aad: group_id too long"
+  ) else if not (msg.epoch < pow2 64) then (
+    internal_failure "message_to_ciphertext_content_aad: epoch too big"
+  ) else if not (Seq.length msg.authenticated_data < pow2 32) then (
+    internal_failure "message_to_ciphertext_content_aad: authenticated_data too long"
+  ) else (
+    return ({
+      group_id = msg.group_id;
+      epoch = u64 msg.epoch;
+      content_type = message_content_type_to_network msg.content_type;
+      authenticated_data = msg.authenticated_data;
+    } <: mls_ciphertext_content_aad_nt)
+  )
+
+val encrypt_ciphertext_content: cs:ciphersuite -> ad:mls_ciphertext_content_aad_nt -> aead_key cs -> aead_nonce cs -> (mls_ciphertext_content_nt ad.content_type) -> result bytes
+let encrypt_ciphertext_content cs ad key nonce pt =
+    aead_encrypt cs key nonce (ps_mls_ciphertext_content_aad.serialize ad) ((ps_mls_ciphertext_content ad.content_type).serialize pt)
 
 val apply_reuse_guard: cs:ciphersuite -> lbytes 4 -> aead_nonce cs -> aead_nonce cs
 let apply_reuse_guard cs reuse_guard nonce =
@@ -226,36 +478,22 @@ let apply_reuse_guard cs reuse_guard nonce =
   let new_nonce_head = Seq.seq_of_list (map2 Lib.IntTypes.logxor (Seq.seq_to_list nonce_head) (Seq.seq_to_list reuse_guard)) in
   Seq.append new_nonce_head nonce_tail
 
-val network_to_encrypted_sender_data: mls_sender_data_nt -> encrypted_sender_data_content
-let network_to_encrypted_sender_data sd =
-  ({
-    sender = Lib.IntTypes.v sd.sender;
-    generation = Lib.IntTypes.v sd.generation;
-    reuse_guard = sd.reuse_guard;
-  })
-
-val network_to_message_ciphertext: mls_ciphertext_nt -> result message_ciphertext
-let network_to_message_ciphertext ct =
-  content_type <-- network_to_message_content_type ct.content_type;
-  return ({
-    group_id = ct.group_id;
-    epoch = Lib.IntTypes.v ct.epoch;
-    content_type = content_type;
-    authenticated_data = ct.authenticated_data;
-    encrypted_sender_data = ct.encrypted_sender_data;
-    ciphertext = ct.ciphertext;
-  })
-
 val message_ciphertext_to_message: #cs:ciphersuite -> (nat -> result (ratchet_output cs)) -> bytes -> message_ciphertext -> result (message & message_auth)
 let message_ciphertext_to_message #cs get_key_nonce sender_data_secret ct =
-  sender_data <-- decrypt_sender_data cs ct sender_data_secret;
-  let sender_data = network_to_encrypted_sender_data sender_data in
-  rs_output <-- get_key_nonce sender_data.generation;
-  let nonce = rs_output.nonce in
-  let key = rs_output.key in
-  let patched_nonce = apply_reuse_guard cs sender_data.reuse_guard nonce in
-  ciphertext_content_bytes <-- decrypt_ciphertext_content cs ct key patched_nonce;
-  ciphertext_content <-- network_to_ciphertext_content ciphertext_content_bytes;
+  sender_data <-- (
+    sender_data_ad <-- message_ciphertext_to_sender_data_aad ct;
+    sender_data <-- decrypt_sender_data cs sender_data_ad (get_ciphertext_sample cs ct.ciphertext) sender_data_secret ct.encrypted_sender_data;
+    return (network_to_encrypted_sender_data sender_data)
+  );
+  ciphertext_content <-- (
+    rs_output <-- get_key_nonce sender_data.generation;
+    let nonce = rs_output.nonce in
+    let key = rs_output.key in
+    let patched_nonce = apply_reuse_guard cs sender_data.reuse_guard nonce in
+    ciphertext_content_ad <-- message_ciphertext_to_ciphertext_content_aad ct;
+    ciphertext_content_network <-- decrypt_ciphertext_content cs ciphertext_content_ad key patched_nonce ct.ciphertext;
+    network_to_ciphertext_content (ciphertext_content_network <: mls_ciphertext_content_nt (message_content_type_to_network ct.content_type))
+  );
   return (({
     group_id = ct.group_id;
     epoch = ct.epoch;
@@ -271,3 +509,43 @@ let message_ciphertext_to_message #cs get_key_nonce sender_data_secret ct =
     confirmation_tag = ciphertext_content.confirmation_tag;
   } <: message_auth))
 
+val message_to_message_ciphertext: #cs:ciphersuite -> ratchet_state cs -> randomness 4 -> bytes -> (message & message_auth) -> result (message_ciphertext & ratchet_state cs)
+let message_to_message_ciphertext #cs ratchet rand sender_data_secret (msg, msg_auth) =
+  let reuse_guard = get_random_bytes rand in
+  ciphertext <-- (
+    key_nonce <-- ratchet_get_key ratchet;
+    let key = key_nonce.key in
+    let patched_nonce = apply_reuse_guard cs reuse_guard key_nonce.nonce in
+    let ciphertext_content: message_ciphertext_content (msg.content_type) = {
+      message_content = msg.message_content;
+      signature = msg_auth.signature;
+      confirmation_tag = msg_auth.confirmation_tag;
+      padding = bytes_empty; //TODO
+    } in
+    ciphertext_content_network <-- ciphertext_content_to_network cs ciphertext_content;
+    ciphertext_content_ad <-- message_to_ciphertext_content_aad msg;
+    encrypt_ciphertext_content cs ciphertext_content_ad key patched_nonce ciphertext_content_network
+  );
+  encrypted_sender_data <-- (
+    if not (msg.sender.sender_type = ST_member) then
+      error "message_to_message_ciphertext: sender is not a member"
+    else (
+      sender_data_ad <-- message_to_sender_data_aad msg;
+      let sender_data = ({
+        sender = msg.sender.sender_id;
+        generation = ratchet.generation;
+        reuse_guard = reuse_guard;
+      }) in
+      sender_data_network <-- encrypted_sender_data_to_network sender_data;
+      encrypt_sender_data cs sender_data_ad (get_ciphertext_sample cs ciphertext) sender_data_secret sender_data_network
+    )
+  );
+  new_ratchet <-- ratchet_next_state ratchet;
+  return ({
+    group_id = msg.group_id;
+    epoch = msg.epoch;
+    content_type = msg.content_type;
+    authenticated_data = msg.authenticated_data;
+    encrypted_sender_data = encrypted_sender_data;
+    ciphertext = ciphertext;
+  }, new_ratchet)
